The beginning of (weak) reducibility. Escape.v goes through

theories/LContexts.v
@@ -1,24 +1,24 @@
 Require Import ssreflect.
-Require Import Coq.Arith.EqNat.
+Require Import Coq.Arith.EqNat PeanoNat.
 From LogRel.AutoSubst Require Import core unscoped Ast Extra.
 From LogRel Require Import Utils.
 
 Notation LCon := (list (prod nat bool)).
 
-Inductive in_LCon : LCon -> nat -> bool -> Prop :=
+Inductive in_LCon : LCon -> nat -> bool -> Type :=
 | in_here_l (l : LCon) {n b} : in_LCon (cons (n,b) l) n b
 | in_there_l {l : LCon} {n b d} : in_LCon l n b -> in_LCon (cons d l) n b.
 
-Inductive not_in_LCon : LCon -> nat -> Prop :=
+Inductive not_in_LCon : LCon -> nat -> Type :=
 | not_in_nil : forall n, not_in_LCon nil n
 | not_in_there : forall {l n m b}, n <> m -> not_in_LCon l n
                                  -> not_in_LCon (cons (m,b) l) n.
 
-Inductive wf_LCon : LCon -> Prop :=
+Inductive wf_LCon : LCon -> Type :=
 | wf_nil : wf_LCon nil
 | wf_cons : forall {l n b}, wf_LCon l -> not_in_LCon l n -> wf_LCon (cons (n,b) l).
 
-Definition le_LCon l l' : Prop :=
+Definition le_LCon l l' : Type :=
   forall n b, in_LCon l n b -> in_LCon l' n b.
 
 Definition le_LCon_refl l : le_LCon l l := fun n b ne => ne.
@@ -90,10 +90,11 @@ Proof.
   - now inversion inl.
   - inversion inl ; subst.
     + inversion inl' ; subst ; trivial.
-      exfalso ; exact (notinLConnotinLCon H H4).
+      exfalso.
+      exact (notinLConnotinLCon n1 H3).
     + inversion inl' ; subst.
-      * exfalso ; exact (notinLConnotinLCon H H4).
-      * exact (IHwfl H4 H5).
+      * exfalso ; exact (notinLConnotinLCon n1 H3).
+      * exact (IHwfl H3 H4).
 Qed.
 
 Lemma decidInLCon l n : (in_LCon l n true) + (in_LCon l n false) + (not_in_LCon l n).
@@ -133,9 +134,9 @@ Definition wfLCons' (l : wfLCon) {n : nat} (d : (not_in_LCon (pi1 l) n) × bool)
 
 Notation " l ',,l' d " := (wfLCons' l d) (at level 20, d at next level).
 
-Definition LCon_le (l l' : LCon) : Prop := forall n b, in_LCon l' n b -> in_LCon l n b.
+Definition LCon_le (l l' : LCon) : Type := forall n b, in_LCon l' n b -> in_LCon l n b.
 
-Definition wfLCon_le (l l' : wfLCon) : Prop :=
+Definition wfLCon_le (l l' : wfLCon) : Type :=
   LCon_le (pi1 l) (pi1 l').
 
 Notation " l ≤ε l' " := (wfLCon_le l l') (at level 40).
@@ -172,4 +173,83 @@ Proof.
   - now eapply LCon_le_step.
   - now eapply in_here_l.
   - exact inl.
+Qed.
+
+
+Fixpoint RemoveElt {l : LCon} {n b} (ne : in_LCon l n b) : LCon
+  := match ne with
+     | in_here_l l => l
+     | @in_there_l l n b d ne => cons d (RemoveElt ne)
+     end.
+
+Lemma Remove_notinLCon {l : LCon} {n m b} (ne : in_LCon l n b) (me : not_in_LCon l m) :
+  not_in_LCon (RemoveElt ne) m.
+Proof.
+  induction ne.
+  - cbn in *.
+    now inversion me.
+  - destruct d ; cbn in *.
+    inversion me ; subst.
+    econstructor.
+    + assumption.
+    + now apply IHne.
+Qed.
+
+Definition wf_RemoveElt {l : wfLCon} {n b} (ne : in_LCon l n b) : wfLCon.
+Proof.
+  exists (RemoveElt ne).
+  destruct l as [l wfl] ; cbn in *.
+  induction ne.
+  - now inversion wfl.
+  - cbn.
+    destruct d.
+    econstructor.
+    + eapply IHne.
+      now inversion wfl.
+    + eapply Remove_notinLCon.
+      now inversion wfl.
+Defined.
+
+Lemma RemoveElt_le {l l' n b} (f : l' ≤ε l) (ne : in_LCon l n b) :
+  (wf_RemoveElt (f n b ne))  ≤ε (wf_RemoveElt ne).
+Proof.
+Admitted.
+  
+Lemma LCon_le_le {l l'} :  l' ≤ε l -> length l <= length l'.
+Proof.
+  intro f.
+  destruct l as [l wfl] ; cbn in *.
+  revert l' f.
+  induction wfl ; intros.
+  - now eapply le_0_n.
+  -
+Admitted.
+
+Fixpoint LCon_newElt (l : LCon) : nat :=
+  match l with
+  | nil => 0
+  | cons (n , b) q => max (LCon_newElt q) (S n)
+  end.
+
+Lemma newElt_newElt_aux (l : LCon) (n : nat) :
+  not_in_LCon l (max (LCon_newElt l) n).
+Proof.
+  revert n.
+  induction l as [ | [n b]] ; intros.
+  - constructor.
+  - cbn.
+    econstructor.
+    + eapply Nat.neq_sym.
+      eapply Nat.lt_neq.
+      eapply Nat.lt_le_trans.
+      eapply Nat.lt_succ_diag_r.
+      etransitivity ; [eapply Nat.le_max_r |..] ; now eapply Nat.le_max_l.
+    + now erewrite <- Nat.max_assoc.
+Qed.
+
+Lemma newElt_newElt (l : LCon) (n : nat) :
+  not_in_LCon l (LCon_newElt l).
+Proof.
+  pose proof (newElt_newElt_aux l 0).
+  now rewrite Nat.max_0_r in H.
 Qed.
