theories/LogicalRelation/Escape.v
@@ -1,4 +1,5 @@
 (** * LogRel.LogicalRelation.Escape: the logical relation implies conversion/typing. *)
+Require Import PeanoNat Nat.
 From Coq Require Import CRelationClasses.
 From LogRel.AutoSubst Require Import core unscoped Ast Extra.
 From LogRel Require Import Utils BasicAst Notations LContexts Context NormalForms GenericTyping LogicalRelation DeclarativeInstance.
@@ -27,6 +28,44 @@ Section Escapes.
     - intros ???? []; gen_typing.
   Qed.
 
+  Lemma Wescape {l wl Γ A} : W[ Γ ||-< l > A ]< wl > -> [Γ |- A]< wl >.
+  Proof.
+    intros [].
+    remember (WN - length wl).
+    revert wl Heqn WRed.
+    induction n.
+    - intros.
+      eapply escape.
+      eapply WRed.
+      + now eapply wfLCon_le_id.
+      + eapply PeanoNat.Nat.sub_0_le.
+        now rewrite Heqn.
+    - intros.
+      unshelve eapply wft_ϝ.
+      + exact (LCon_newElt wl).
+      + now eapply newElt_newElt.
+      + eapply IHn.
+        * cbn.
+          erewrite PeanoNat.Nat.sub_succ_r.
+          rewrite <- Heqn.
+          reflexivity.
+        * intros.
+          eapply WRed ; try eassumption.
+          eapply wfLCon_le_trans ; try eassumption.
+          eapply LCon_le_step.
+          now eapply wfLCon_le_id.
+      + eapply IHn.
+        * cbn.
+          erewrite PeanoNat.Nat.sub_succ_r.
+          rewrite <- Heqn.
+          reflexivity.
+        * intros.
+          eapply WRed ; try eassumption.
+          eapply wfLCon_le_trans ; try eassumption.
+          eapply LCon_le_step.
+          now eapply wfLCon_le_id.
+  Qed.
+         
   Lemma escapeEq {l wl Γ A B} (lr : [Γ ||-< l > A]< wl >) :
       [ Γ ||-< l > A ≅ B | lr ]< wl > ->
       [Γ |- A ≅ B]< wl >.
@@ -45,6 +84,55 @@ Section Escapes.
     + intros ???? [] []; gen_typing.
   Qed.
 
+  Lemma WescapeEq {l wl Γ A B} (lr : W[Γ ||-< l > A]< wl >) :
+      W[ Γ ||-< l > A ≅ B | lr ]< wl > ->
+      [Γ |- A ≅ B]< wl >.
+  Proof.
+    intros [].
+    destruct lr as [WN WRed].
+    remember ((max WN WNEq) - length wl).
+    revert wl Heqn WRed WRedEq.
+    induction n ; intros.
+    - eapply escapeEq.
+      unshelve eapply WRedEq.
+      + now eapply wfLCon_le_id.
+      + etransitivity.
+        eapply Nat.le_max_l.
+        eapply Nat.sub_0_le.
+        now rewrite Heqn.
+      + etransitivity.
+        eapply Nat.le_max_r.
+        eapply Nat.sub_0_le.
+        now rewrite Heqn.
+    - unshelve eapply convty_ϝ.
+      + exact (LCon_newElt wl).
+      + now eapply newElt_newElt.
+      + unshelve eapply IHn.
+        * intros.
+          unshelve eapply WRed ; try eassumption.
+          eapply wfLCon_le_trans ; try eassumption.
+          eapply LCon_le_step.
+          now eapply wfLCon_le_id.
+        * cbn.
+          erewrite PeanoNat.Nat.sub_succ_r.
+          rewrite <- Heqn.
+          reflexivity.
+        * intros.
+          now unshelve eapply WRedEq.
+      + unshelve eapply IHn.
+        * intros.
+          unshelve eapply WRed ; try eassumption.
+          eapply wfLCon_le_trans ; try eassumption.
+          eapply LCon_le_step.
+          now eapply wfLCon_le_id.
+        * cbn.
+          erewrite PeanoNat.Nat.sub_succ_r.
+          rewrite <- Heqn.
+          reflexivity.
+        * intros.
+          now unshelve eapply WRedEq.
+Qed.
+
   Definition escapeTerm {l wl Γ t A} (lr : [Γ ||-< l > A ]< wl >) :
     [Γ ||-< l > t : A | lr ]< wl > ->
     [Γ |- t : A]< wl >.
@@ -61,6 +149,55 @@ Section Escapes.
     - intros ???? [] []; gen_typing.
   Qed.
 
+  Definition WescapeTerm {l wl Γ t A} (lr : W[Γ ||-< l > A ]< wl >) :
+    W[Γ ||-< l > t : A | lr ]< wl > ->
+    [Γ |- t : A]< wl >.
+  Proof.
+   intros [].
+    destruct lr as [WN WRed].
+    remember ((max WN WNTm) - length wl).
+    revert wl Heqn WRed WRedTm.
+    induction n ; intros.
+    - eapply escapeTerm.
+      unshelve eapply WRedTm.
+      + now eapply wfLCon_le_id.
+      + etransitivity.
+        eapply Nat.le_max_l.
+        eapply Nat.sub_0_le.
+        now rewrite Heqn.
+      + etransitivity.
+        eapply Nat.le_max_r.
+        eapply Nat.sub_0_le.
+        now rewrite Heqn.
+    - unshelve eapply ty_ϝ.
+      + exact (LCon_newElt wl).
+      + now eapply newElt_newElt.
+      + unshelve eapply IHn.
+        * intros.
+          unshelve eapply WRed ; try eassumption.
+          eapply wfLCon_le_trans ; try eassumption.
+          eapply LCon_le_step.
+          now eapply wfLCon_le_id.
+        * cbn.
+          erewrite PeanoNat.Nat.sub_succ_r.
+          rewrite <- Heqn.
+          reflexivity.
+        * intros.
+          now unshelve eapply WRedTm.
+      + unshelve eapply IHn.
+        * intros.
+          unshelve eapply WRed ; try eassumption.
+          eapply wfLCon_le_trans ; try eassumption.
+          eapply LCon_le_step.
+          now eapply wfLCon_le_id.
+        * cbn.
+          erewrite PeanoNat.Nat.sub_succ_r.
+          rewrite <- Heqn.
+          reflexivity.
+        * intros.
+          now unshelve eapply WRedTm.
+  Qed.
+  
   Definition escapeEqTerm {l wl Γ t u A} (lr : [Γ ||-< l > A ]< wl >) :
     [Γ ||-< l > t ≅ u : A | lr ]< wl > ->
     [Γ |- t ≅ u : A]< wl >.
@@ -83,6 +220,55 @@ Section Escapes.
       eapply convtm_exp; tea; gen_typing.
   Qed.
 
+  Definition WescapeEqTerm {l wl Γ t u A} (lr : W[Γ ||-< l > A ]< wl >) :
+    W[Γ ||-< l > t ≅ u : A | lr ]< wl > ->
+    [Γ |- t ≅ u : A]< wl >.
+  Proof.
+    intros [].
+    destruct lr as [WN WRed].
+    remember ((max WN WNTmEq) - length wl).
+    revert wl Heqn WRed WRedTmEq.
+    induction n ; intros.
+    - eapply escapeEqTerm.
+      unshelve eapply WRedTmEq.
+      + now eapply wfLCon_le_id.
+      + etransitivity.
+        eapply Nat.le_max_l.
+        eapply Nat.sub_0_le.
+        now rewrite Heqn.
+      + etransitivity.
+        eapply Nat.le_max_r.
+        eapply Nat.sub_0_le.
+        now rewrite Heqn.
+    - unshelve eapply convtm_ϝ.
+      + exact (LCon_newElt wl).
+      + now eapply newElt_newElt.
+      + unshelve eapply IHn.
+        * intros.
+          unshelve eapply WRed ; try eassumption.
+          eapply wfLCon_le_trans ; try eassumption.
+          eapply LCon_le_step.
+          now eapply wfLCon_le_id.
+        * cbn.
+          erewrite PeanoNat.Nat.sub_succ_r.
+          rewrite <- Heqn.
+          reflexivity.
+        * intros.
+          now unshelve eapply WRedTmEq.
+      + unshelve eapply IHn.
+        * intros.
+          unshelve eapply WRed ; try eassumption.
+          eapply wfLCon_le_trans ; try eassumption.
+          eapply LCon_le_step.
+          now eapply wfLCon_le_id.
+        * cbn.
+          erewrite PeanoNat.Nat.sub_succ_r.
+          rewrite <- Heqn.
+          reflexivity.
+        * intros.
+          now unshelve eapply WRedTmEq.
+  Qed.
+  
   Lemma escapeConv {l wl Γ A} (RA : [Γ ||-<l> A]< wl >) :
     forall B,
     [Γ ||-<l> A ≅ B | RA]< wl > ->
@@ -96,6 +282,58 @@ Section Escapes.
     - intros * []; gen_typing.
     - intros * []; gen_typing.
   Qed.
+
+  Lemma WescapeConv {l wl Γ A} (RA : W[Γ ||-<l> A]< wl >) :
+    forall B,
+    W[Γ ||-<l> A ≅ B | RA]< wl > ->
+    [Γ |- B]< wl >.
+  Proof.
+    intros B [].
+    destruct RA as [WN WRed].
+    remember ((max WN WNEq) - length wl).
+    revert wl Heqn WRed WRedEq.
+    induction n ; intros.
+    - eapply escapeConv.
+      unshelve eapply WRedEq.
+      + now eapply wfLCon_le_id.
+      + etransitivity.
+        eapply Nat.le_max_l.
+        eapply Nat.sub_0_le.
+        now rewrite Heqn.
+      + etransitivity.
+        eapply Nat.le_max_r.
+        eapply Nat.sub_0_le.
+        now rewrite Heqn.
+    - unshelve eapply wft_ϝ.
+      + exact (LCon_newElt wl).
+      + now eapply newElt_newElt.
+      + unshelve eapply IHn.
+        * intros.
+          unshelve eapply WRed ; try eassumption.
+          eapply wfLCon_le_trans ; try eassumption.
+          eapply LCon_le_step.
+          now eapply wfLCon_le_id.
+        * cbn.
+          erewrite PeanoNat.Nat.sub_succ_r.
+          rewrite <- Heqn.
+          reflexivity.
+        * intros.
+          now unshelve eapply WRedEq.
+      + unshelve eapply IHn.
+        * intros.
+          unshelve eapply WRed ; try eassumption.
+          eapply wfLCon_le_trans ; try eassumption.
+          eapply LCon_le_step.
+          now eapply wfLCon_le_id.
+        * cbn.
+          erewrite PeanoNat.Nat.sub_succ_r.
+          rewrite <- Heqn.
+          reflexivity.
+        * intros.
+          now unshelve eapply WRedEq.
+  Qed.
+
+  
   
 End Escapes.
 
